feat: finished main verification of checkLambda

Lean4Lean/Instantiate.lean
@@ -1,4 +1,5 @@
 import Lean.Expr
+import Lean.LocalContext
 
 namespace Lean
 namespace Expr
@@ -8,7 +9,7 @@ def cheapBetaReduce (e : Expr) : Expr := Id.run do
   let fn := e.getAppFn
   if !fn.isLambda then return e
   let args := e.getAppArgs
-  let cont i fn :=
+  let rec cont i fn :=
     if !fn.hasLooseBVars then
       mkAppRange fn i args.size args
     else if let .bvar n := fn then
@@ -44,6 +45,30 @@ def liftLooseBVars' (e : @& Expr) (s d : @& Nat) : Expr :=
   | e@(.lit _) => e
 
 /--
+Lower the loose bound variables `>= s` in `e` by `d`.
+That is, a loose bound variable `bvar i` with `i >= s` is mapped to `bvar (i-d)`.
+
+Remark: if `s < d`, then the result is `e`.
+-/
+@[implemented_by lowerLooseBVars]
+def lowerLooseBVars' (e : @& Expr) (s d : @& Nat) : Expr :=
+  if s < d then e else
+  match e with
+  | .bvar i => .bvar (if i < s then i else i - d)
+  | .mdata m e => .mdata m (lowerLooseBVars' e s d)
+  | .proj n i e => .proj n i (lowerLooseBVars' e s d)
+  | .app f a => .app (lowerLooseBVars' f s d) (lowerLooseBVars' a s d)
+  | .lam n t b bi => .lam n (lowerLooseBVars' t s d) (lowerLooseBVars' b (s+1) d) bi
+  | .forallE n t b bi => .forallE n (lowerLooseBVars' t s d) (lowerLooseBVars' b (s+1) d) bi
+  | .letE n t v b bi =>
+    .letE n (lowerLooseBVars' t s d) (lowerLooseBVars' v s d) (lowerLooseBVars' b (s+1) d) bi
+  | e@(.const ..)
+  | e@(.sort _)
+  | e@(.fvar _)
+  | e@(.mvar _)
+  | e@(.lit _) => e
+
+/--
 Instantiates loose bound variable `0` in `e` using the expression `subst`,
 where in particular a loose `Expr.bvar i` at binding depth `d` is instantiated with `subst` if `i = d`,
 and otherwise it is replaced with `Expr.bvar (i - 1)`; non-loose bound variables are not touched.
@@ -67,6 +92,10 @@ where
   | e@(.mvar _), _
   | e@(.lit _), _ => e
 
+@[simp] def instantiateList : Expr → List Expr → (k :_:= 0) → Expr
+  | e, [], _ => e
+  | e, a :: as, k => instantiateList (instantiate1'.go a e k) as k
+
 /--
 Instantiates the loose bound variables in `e` using the `subst` array,
 where a loose `Expr.bvar i` at "binding depth" `d` is instantiated with `subst[i - d]` if `0 <= i - d < subst.size`,
@@ -74,11 +103,7 @@ and otherwise it is replaced with `Expr.bvar (i - subst.size)`; non-loose bound 
 -/
 @[implemented_by instantiate]
 def instantiate' (e : @& Expr) (subst : @& Array Expr) : Expr :=
-  go e subst.toList
-where
-  go : Expr → List Expr → Expr
-  | e, [] => e
-  | e, a :: as => go (e.instantiate1' a) as
+  instantiateList e subst.toList
 
 @[implemented_by instantiateRev]
 def instantiateRev' (e : @& Expr) (subst : @& Array Expr) : Expr :=
@@ -92,6 +117,93 @@ def instantiateRange' (e : @& Expr) (beginIdx endIdx : @& Nat) (subst : @& Array
 def instantiateRevRange' (e : @& Expr) (beginIdx endIdx : @& Nat) (subst : @& Array Expr) : Expr :=
   e.instantiateRev' (subst.extract beginIdx endIdx)
 
-theorem instantiateRev_push {e : Expr} {subst a} :
-    instantiateRev' e (subst.push a) = instantiateRev' (e.instantiate1' a) subst := by
-  let ⟨subst⟩ := subst; simp [instantiateRev', instantiate', instantiate'.go]
+def abstractFVar (v : FVarId) : Expr → (k :_:= 0) → Expr
+  | .bvar i, d => .bvar (if i < d then i else i + 1)
+  | e@(.fvar v'), d => if v == v' then .bvar d else e
+  | .mdata m e, d => .mdata m (abstractFVar v e d)
+  | .proj s i e, d => .proj s i (abstractFVar v e d)
+  | .app f a, d => .app (abstractFVar v f d) (abstractFVar v a d)
+  | .lam n t b bi, d => .lam n (abstractFVar v t d) (abstractFVar v b (d+1)) bi
+  | .forallE n t b bi, d => .forallE n (abstractFVar v t d) (abstractFVar v b (d+1)) bi
+  | .letE n t val b bi, d =>
+    .letE n (abstractFVar v t d) (abstractFVar v val d) (abstractFVar v b (d+1)) bi
+  | e@(.const ..), _
+  | e@(.sort _), _
+  | e@(.mvar _), _
+  | e@(.lit _), _ => e
+
+-- this can be defined but it's not used in the kernel
+opaque abstract1Other : Expr → Expr → (k :_:= 0) → Expr
+
+def abstract1 (e : Expr) : Expr → (k :_:= 0) → Expr
+  | .fvar a, k => abstractFVar a e k
+  | a, k => abstract1Other a e k
+
+@[simp] def abstractList : Expr → List Expr → (k :_:= 0) → Expr
+  | e, [], _ => e
+  | e, a :: as, k => abstractList (abstract1 e a k) as k
+
+@[simp] def abstractRevList : Expr → List Expr → (k :_:= 0) → Expr
+  | e, [], _ => e
+  | e, a :: as, k => abstract1 (abstractRevList e as k) a k
+
+/-- Replace free (or meta) variables `xs` with loose bound variables,
+with `xs` ordered from outermost to innermost de Bruijn index.
+
+For example, `e := f x y` with `xs := #[x, y]` goes to `f #1 #0`,
+whereas `e := f x y` with `xs := #[y, x]` goes to `f #0 #1`. -/
+@[implemented_by abstract]
+def abstract' (e : @& Expr) (xs : @& Array Expr) : Expr :=
+  e.abstractList xs.toList
+
+/-- Similar to `abstract`, but consider only the first `min n xs.size` entries in `xs`. -/
+@[implemented_by abstractRange]
+def abstractRange' (e : @& Expr) (n : @& Nat) (xs : @& Array Expr) : Expr :=
+  e.abstract' (xs.extract 0 n)
+
+@[implemented_by hasLooseBVar]
+def hasLooseBVar' : (e : @& Expr) → (bvarIdx : @& Nat) → Bool
+  | .bvar i, d => i = d
+  | .mdata _ e, d
+  | .proj _ _ e, d => hasLooseBVar' e d
+  | .app f a, d => hasLooseBVar' f d || hasLooseBVar' a d
+  | .lam _ t b _, d
+  | .forallE _ t b _, d => hasLooseBVar' t d || hasLooseBVar' b (d+1)
+  | .letE _ t v b _, d => hasLooseBVar' t d || hasLooseBVar' v d || hasLooseBVar' b (d+1)
+  | .const .., _
+  | .sort _, _
+  | .fvar _, _
+  | .mvar _, _
+  | .lit _, _ => false
+
+end Expr
+
+@[inline] def LocalContext.mkBinding' (isLambda : Bool) (lctx : LocalContext) (xs : Array Expr) (b : Expr) : Expr :=
+  let b := b.abstract' xs
+  xs.size.foldRev (init := b) fun i _ b =>
+    let x := xs[i]
+    match lctx.findFVar? x with
+    | some (.cdecl _ _ n ty bi _)  =>
+      let ty := ty.abstractRange' i xs
+      if isLambda then
+        Lean.mkLambda n bi ty b
+      else
+        Lean.mkForall n bi ty b
+    | some (.ldecl _ _ n ty val nonDep _) =>
+      if b.hasLooseBVar' 0 then
+        let ty  := ty.abstractRange' i xs
+        let val := val.abstractRange' i xs
+        mkLet n ty val b nonDep
+      else
+        b.lowerLooseBVars' 1 1
+    | none => panic! "unknown free variable"
+
+/-- Creates the expression `fun x₁ .. xₙ => b` for free variables `xs = #[x₁, .., xₙ]`,
+suitably abstracting `b` and the types for each of the `xᵢ`. -/
+def LocalContext.mkLambda' (lctx : LocalContext) (xs : Array Expr) (b : Expr) : Expr :=
+  mkBinding' true lctx xs b
+
+/-- Creates the expression `(x₁:α₁) → .. → (xₙ:αₙ) → b` for free variables `xs = #[x₁, .., xₙ]`,
+suitably abstracting `b` and the types for each of the `xᵢ`, `αᵢ`. -/
+def LocalContext.mkForall' (lctx : LocalContext) (xs : Array Expr) (b : Expr) : Expr :=
+  mkBinding' false lctx xs b
