Lean4Lean/Verify/LocalContext.lean
@@ -1,5 +1,121 @@
 import Lean4Lean.Verify.Axioms
+import Lean4Lean.Verify.Expr
 import Lean4Lean.Verify.Typing.Expr
+
+namespace Lean.LocalContext
+
+noncomputable def toList (lctx : LocalContext) : List LocalDecl :=
+  lctx.decls.toList'.reverse.filterMap id
+
+noncomputable def fvars (lctx : LocalContext) : List FVarId :=
+  lctx.toList.map (·.fvarId)
+
+def mkBindingList1 (isLambda : Bool) (lctx : LocalContext)
+    (xs : List FVarId) (x : FVarId) (b : Expr) : Expr :=
+  match lctx.find? x with
+  | some (.cdecl _ _ n ty bi _) =>
+    let ty := ty.abstractList (xs.map .fvar)
+    if isLambda then
+      .lam n ty b bi
+    else
+      .forallE n ty b bi
+  | some (.ldecl _ _ n ty val nonDep _) =>
+    if b.hasLooseBVar' 0 then
+      let ty  := ty.abstractList (xs.map .fvar)
+      let val := val.abstractList (xs.map .fvar)
+      .letE n ty val b nonDep
+    else
+      b.lowerLooseBVars' 1 1
+  | none => panic! "unknown free variable"
+
+def mkBindingList (isLambda : Bool) (lctx : LocalContext) (xs : List FVarId) (b : Expr) : Expr :=
+  core (b.abstractList (xs.map .fvar))
+where
+  core := go xs.reverse
+  go : List FVarId → Expr → Expr
+  | [], b => b
+  | x :: xs, b => go xs (mkBindingList1 isLambda lctx xs.reverse x b)
+
+theorem mkBinding'_eq :
+    mkBinding' isLambda lctx ⟨xs.map .fvar⟩ b = mkBindingList isLambda lctx xs b := by
+  simp only [mkBinding', List.getElem_toArray, Expr.abstractRange',
+    Expr.abstract', List.extract_toArray, Nat.sub_zero, List.drop_zero]; dsimp only [Array.size]
+  simp only [← List.map_take, List.getElem_map]
+  simp only [List.getElem_eq_getElem?_get, Option.get_eq_getD (fallback := default)]
+  change Nat.foldRev _ (fun i x =>
+    mkBindingList1 isLambda lctx (xs.take i) (xs[i]?.getD default)) .. = mkBindingList.go ..
+  rw [List.length_map]; generalize eq : xs.length = n
+  generalize b.abstractList (xs.map .fvar) = b
+  induction n generalizing xs b with
+  | zero => let [] := xs; simp [mkBindingList.go]
+  | succ n ih =>
+    obtain rfl | ⟨xs, a, rfl⟩ := List.eq_nil_or_concat xs; · cases eq
+    simp at eq ⊢; subst eq
+    simp +contextual only [Nat.le_of_lt, List.take_append_of_le_length,
+      List.getElem?_append_left, mkBindingList.go, ih]; simp
+
+theorem mkBindingList1_abstract {xs : List FVarId}
+    (hx : lctx.find? x = some decl) (nd : (a :: xs).Nodup) :
+    (mkBindingList1 isLambda lctx xs x b).abstractFVar a xs.length =
+    mkBindingList1 isLambda lctx (a :: xs) x (b.abstractFVar a (xs.length + 1)) := by
+  have (e) := Nat.zero_add _ ▸ Expr.abstractFVar_abstractList' (k := 0) (e := e) nd
+  simp [mkBindingList1, hx]; cases decl with simp
+  | cdecl _ _ _ ty =>
+    split <;> simp [Expr.abstractFVar, Expr.abstract1, this]
+  | ldecl =>
+    have := Expr.abstractFVar_hasLooseBVar a b (xs.length + 1) 0
+    simp at this; simp [this]; clear this
+    split
+    · simp [Expr.abstractFVar, Expr.abstract1, this]
+    · rename_i h; simp at h
+      rw [Expr.abstractFVar_lower h (Nat.zero_le _)]
+
+theorem mkBindingList_core_cons {xs : List FVarId} {b : Expr}
+    (hx : ∀ x ∈ xs, ∃ decl, lctx.find? x = some decl) (nd : (a :: xs).Nodup) :
+    mkBindingList.core isLambda lctx (a :: xs) (b.abstractFVar a xs.length) =
+    mkBindingList1 isLambda lctx [] a
+      ((mkBindingList.core isLambda lctx xs b).abstractFVar a) := by
+  obtain ⟨xs, rfl⟩ : ∃ xs', List.reverse xs' = xs := ⟨_, List.reverse_reverse _⟩
+  simp [mkBindingList.core] at *
+  induction xs generalizing b with
+  | nil => simp [mkBindingList.go]
+  | cons c xs ih =>
+    simp at hx nd ih
+    let ⟨decl, eq⟩ := hx.1
+    simp [← List.map_reverse, mkBindingList.go]
+    rw [← xs.length_reverse, ← mkBindingList1_abstract eq (by simp [*])]
+    simp [ih hx.2 nd.1.2 nd.2.2]
+
+@[simp] theorem mkBindingList_nil : mkBindingList isLambda lctx [] b = b := rfl
+
+theorem mkBindingList_cons
+    (hx : ∀ x ∈ xs, ∃ decl, lctx.find? x = some decl) (nd : (a :: xs).Nodup) :
+    mkBindingList isLambda lctx (a :: xs) b =
+    mkBindingList1 isLambda lctx [] a ((mkBindingList isLambda lctx xs b).abstractFVar a) := by
+  simp [Expr.abstractList_append, Expr.abstract1, mkBindingList]
+  rw [← Expr.abstractFVar_abstractList' nd]
+  rw [Nat.zero_add, mkBindingList_core_cons hx nd]
+
+theorem mkBindingList_eq_fold
+    (hx : ∀ x ∈ xs, ∃ decl, lctx.find? x = some decl) (nd : xs.Nodup) :
+    mkBindingList isLambda lctx xs b =
+    xs.foldr (fun a e => mkBindingList1 isLambda lctx [] a (e.abstractFVar a)) b := by
+  induction xs <;> simp_all [mkBindingList_cons]
+
+theorem mkBindingList1_congr (H : lctx₁.find? x = lctx₂.find? x) :
+    mkBindingList1 isLambda lctx₁ xs x b = mkBindingList1 isLambda lctx₂ xs x b := by
+  simp [mkBindingList1, H]
+
+theorem mkBindingList_congr
+    (H : ∀ x ∈ xs, lctx₁.find? x = lctx₂.find? x) :
+    mkBindingList isLambda lctx₁ xs b = mkBindingList isLambda lctx₂ xs b := by
+  obtain ⟨xs, rfl⟩ : ∃ xs', List.reverse xs' = xs := ⟨_, List.reverse_reverse _⟩
+  simp [mkBindingList, mkBindingList.core] at *
+  generalize b.abstractList _ = b
+  induction xs generalizing b <;> simp_all [mkBindingList.go]
+  simp [mkBindingList1_congr H.1]
+
+end Lean.LocalContext
 
 namespace Lean4Lean
 
@@ -7,12 +123,6 @@ open Lean
 open scoped List
 
 attribute [-simp] List.filterMap_reverse
-
-noncomputable def _root_.Lean.LocalContext.toList (lctx : LocalContext) : List LocalDecl :=
-  lctx.decls.toList'.reverse.filterMap id
-
-noncomputable def _root_.Lean.LocalContext.fvars (lctx : LocalContext) : List FVarId :=
-  lctx.toList.map (·.fvarId)
 
 variable (env : VEnv) (Us : List Name) (Δ : VLCtx) in
 inductive TrLocalDecl : LocalDecl → VLocalDecl → Prop
@@ -80,6 +190,9 @@ theorem TrLCtx.find?_isSome (H : TrLCtx env Us lctx Δ) :
 theorem TrLCtx.find?_eq_some (H : TrLCtx env Us lctx Δ) :
     (∃ d, lctx.find? fv = some d) ↔ fv ∈ Δ.fvars := by
   rw [← Option.isSome_iff_exists, H.find?_isSome, Option.isSome_iff_exists, VLCtx.find?_eq_some]
+
+theorem TrLCtx.find?_eq_none (H : TrLCtx env Us lctx Δ) :
+    lctx.find? fv = none ↔ ¬fv ∈ Δ.fvars := by simp [← H.find?_eq_some]
 
 theorem TrLCtx.contains (H : TrLCtx env Us lctx Δ) : lctx.contains fv ↔ fv ∈ Δ.fvars := by
   rw [LocalContext.contains, PersistentHashMap.find?_isSome, Option.isSome_iff_exists]
