Lean4Lean/Verify/TypeChecker/Theorems.lean
@@ -11,11 +11,70 @@ open Lean
 
 def Methods.WF : Methods → Prop := sorry
 
+inductive MLCtx where
+  | nil : MLCtx
+  | vlam (id : FVarId) (name : Name) (ty : Expr) (ty' : VExpr) (bi : BinderInfo) :
+    MLCtx → MLCtx
+
+@[simp] def MLCtx.vlctx : MLCtx → VLCtx
+  | .nil => []
+  | .vlam id _ _ ty _ c => (some id, .vlam ty) :: c.vlctx
+
+def MLCtx.lctx : MLCtx → LocalContext
+  | .nil => {}
+  | .vlam id name ty _ bi c => c.lctx.mkLocalDecl id name ty bi
+
+@[simp] def MLCtx.length : MLCtx → Nat
+  | .nil => 0
+  | .vlam _ _ _ _ _ c => c.length + 1
+
+@[simp] def MLCtx.fvarRevList (c : MLCtx) (n) (hn : n ≤ c.length) : List FVarId :=
+  match n, c, hn with
+  | 0, _, _ => []
+  | n+1, .vlam id _ _ _ _ c, h =>
+    id :: c.fvarRevList n (Nat.le_of_succ_le_succ h)
+termination_by structural n
+
+@[simp] def MLCtx.dropN (c : MLCtx) (n) (hn : n ≤ c.length) : MLCtx :=
+  match n, c, hn with
+  | 0, c, _ => c
+  | n+1, .vlam _ _ _ _ _ c, h =>
+      c.dropN n (Nat.le_of_succ_le_succ h)
+termination_by structural n
+
+@[simp] def MLCtx.findDecl? (c : MLCtx) (x : FVarId) : Option LocalDecl :=
+  match c with
+  | .nil => none
+  | .vlam v name ty _ bi c =>
+    if x == v then some (.cdecl c.length v name ty bi default) else c.findDecl? x
+
+def MLCtx.WF (env : VEnv) (Us : List Name) : MLCtx → Prop
+  | .nil => True
+  | .vlam fv _ ty ty' _ c =>
+    c.WF env Us ∧ c.lctx.find? fv = none ∧
+    TrExpr env Us c.vlctx ty ty' ∧
+    env.IsType Us.length c.vlctx.toCtx ty'
+
+theorem MLCtx.WF.tr : ∀ {c : MLCtx}, c.WF env Us → TrLCtx env Us c.lctx c.vlctx
+  | .nil, _ => .nil
+  | .vlam .., ⟨h1, h2, h3, h4⟩ => .mkLocalDecl h1.tr h2 h3 h4
+
+theorem MLCtx.noBV (c : MLCtx) : c.vlctx.NoBV := by
+  induction c <;> trivial
+
 structure VContext extends Context where
   venv : VEnv
   venv_wf : VEnv.WF venv
   trenv : TrEnv safety env venv
-  vlctx : VLCtx
+  mlctx : MLCtx
+  mlctx_wf : mlctx.WF venv lparams
+  lctx_eq : mlctx.lctx = lctx
+
+@[simp] abbrev VContext.lctx' (c : VContext) := c.mlctx.lctx
+@[simp] abbrev VContext.vlctx (c : VContext) := c.mlctx.vlctx
+
+theorem VContext.trlctx (c : VContext) : TrLCtx c.venv c.lparams c.lctx' c.vlctx :=
+  c.mlctx_wf.tr
 
 nonrec abbrev VContext.TrExpr (c : VContext) : Expr → VExpr → Prop :=
   TrExpr c.venv c.lparams c.vlctx
@@ -25,22 +84,39 @@ nonrec abbrev VContext.HasType (c : VContext) : VExpr → VExpr → Prop :=
   c.venv.HasType c.lparams.length c.vlctx.toCtx
 nonrec abbrev VContext.IsDefEqU (c : VContext) : VExpr → VExpr → Prop :=
   c.venv.IsDefEqU c.lparams.length c.vlctx.toCtx
+nonrec abbrev VContext.TrLCtx (c : VContext) : Prop :=
+  TrLCtx c.venv c.lparams c.lctx' c.vlctx
+
+class VContext.MLCWF (c : VContext) (m : MLCtx) : Prop where
+  wf : m.WF c.venv c.lparams
+
+instance (c : VContext) : c.MLCWF c.mlctx := ⟨c.mlctx_wf⟩
 
 structure VState extends State where
 
 class VState.WF (c : VContext) (s : VState) where
-  trctx : TrLCtx c.venv c.lparams c.lctx c.vlctx
-  vlctx_wf : OnCtx c.vlctx.toCtx (c.venv.IsType c.lparams.length)
+  trctx : c.TrLCtx
   ngen_wf : ∀ fv ∈ c.vlctx.fvars, s.ngen.Reserves fv
+
+theorem VState.WF.find?_eq_none {id}
+    (wf : VState.WF c s) (H : ¬s.ngen.Reserves id) : c.lctx'.find? id = none :=
+  wf.trctx.find?_eq_none.2 fun h => H (wf.ngen_wf _ h)
 
 def VState.LE (s₁ s₂ : VState) : Prop :=
   s₁.ngen ≤ s₂.ngen
 
 theorem VState.LE.rfl {s : VState} : s.LE s := NameGenerator.LE.rfl
 
-theorem VState.LE.trans {s₁ : VState} {s₂ : VState} {s₃ : VState}
-    (h₁ : s₁.LE s₂) (h₂ : s₂.LE s₃) : s₁.LE s₃ :=
+theorem VState.LE.trans {s₁ s₂ s₃ : VState} (h₁ : s₁.LE s₂) (h₂ : s₂.LE s₃) : s₁.LE s₃ :=
   NameGenerator.LE.trans h₁ h₂
+
+theorem VState.LE.reservesV {s₁ s₂ : VState} (h : s₁.LE s₂) {{fv}} :
+    s₁.ngen.Reserves fv → s₂.ngen.Reserves fv :=
+  (·.mono h)
+
+theorem VState.LE.reserves {s₁ s₂ : VState} (h : s₁.LE s₂) {{e}} :
+    FVarsIn s₁.ngen.Reserves e → FVarsIn s₂.ngen.Reserves e :=
+  (·.mono h.reservesV)
 
 def M.WF (c : VContext) (vs : VState) (x : M α) (Q : α → VState → Prop) : Prop :=
   vs.WF c → ∀ a s', x c.toContext vs.toState = .ok (a, s') →
@@ -87,44 +163,133 @@ theorem RecM.WF.le {c : VContext} {s : VState} {Q R} {x : RecM α}
     x.WF c s R := fun _ h => (h1 _ h).le H
 
 theorem mkFreshId.WF {c : VContext} {s : VState} :
-    M.WF c s mkFreshId fun a s' => s'.ngen.Reserves ⟨a⟩ ∧ c.lctx.find? ⟨a⟩ = none :=
+    M.WF c s mkFreshId fun a s' => s'.ngen.Reserves ⟨a⟩ ∧ ¬s.ngen.Reserves ⟨a⟩ :=
   sorry
 
 theorem getLCtx.WF {c : VContext} {s : VState} :
-    M.WF c s getLCtx fun a s' => c.lctx = a ∧ s = s' := by
-  rintro wf _ _ ⟨⟩; exact ⟨_, rfl, .rfl, wf, rfl, rfl⟩
+    M.WF c s getLCtx fun a s' => c.lctx' = a ∧ s = s' := by
+  rintro wf _ _ ⟨⟩; exact ⟨_, rfl, .rfl, wf, c.lctx_eq, rfl⟩
 
 theorem RecM.WF.getLCtx {c : VContext} {s : VState} {f : LocalContext → RecM α} {Q}
-    (H : WF c s (f c.lctx) Q) : (getLCtx >>= f).WF c s Q :=
+    (H : WF c s (f c.lctx') Q) : (getLCtx >>= f).WF c s Q :=
   getLCtx.WF.lift.bind <| by rintro _ _ _ ⟨rfl, rfl⟩; exact H
+
+theorem getNGen.WF {c : VContext} {s : VState} :
+    M.WF c s getNGen fun a s' => s.ngen = a ∧ s = s' := by
+  rintro wf _ _ ⟨⟩; exact ⟨_, rfl, .rfl, wf, rfl, rfl⟩
+
+theorem M.WF.getNGen {c : VContext} {s : VState} {f : NameGenerator → M α} {Q}
+    (H : WF c s (f s.ngen) Q) : (getNGen >>= f).WF c s Q :=
+  getNGen.WF.bind <| by rintro _ _ _ ⟨rfl, rfl⟩; exact H
+
+theorem RecM.WF.getNGen {c : VContext} {s : VState} {f : NameGenerator → RecM α} {Q}
+    (H : WF c s (f s.ngen) Q) : (getNGen >>= f).WF c s Q :=
+  getNGen.WF.lift.bind <| by rintro _ _ _ ⟨rfl, rfl⟩; exact H
 
 theorem RecM.WF.stateWF {c : VContext} {s : VState} {x : RecM α} {Q}
     (H : s.WF c → WF c s x Q) : WF c s x Q :=
   fun _ h wf => H wf _ h wf
 
-def VContext.pushLDecl (c : VContext)
-    (id : FVarId) (name : Name) (ty : Expr) (ty' : VExpr) (bi : BinderInfo) : VContext :=
+def VContext.withMLC (c : VContext) (m : MLCtx) [wf : c.MLCWF m] : VContext :=
   { c with
-    vlctx := (some id, .vlam ty') :: c.vlctx
-    lctx := c.lctx.mkLocalDecl id name ty bi }
+    mlctx := m
+    mlctx_wf := wf.1
+    lctx := m.lctx
+    lctx_eq := rfl }
 
-theorem RecM.WF.withLam {c : VContext} {s : VState} {f : RecM α} {Q}
-    {id name ty ty' bi}
-    (h0 : s.ngen.Reserves id)
-    (h1 : c.lctx.find? id = none)
-    (h2 : c.TrExpr ty ty')
-    (h3 : c.IsType ty')
-    (H : WF (c.pushLDecl id name ty ty' bi) s f Q) :
-    (Inner.withLCtx (c.lctx.mkLocalDecl id name ty bi) f).WF c s Q := by
-  intro _ h wf a s' e
-  have : VState.WF (c.pushLDecl id name ty ty' bi) s := {
-    ngen_wf := by simpa [VContext.pushLDecl] using ⟨h0, wf.ngen_wf⟩
-    trctx := wf.trctx.mkLocalDecl h1 h2 h3
-    vlctx_wf := ⟨wf.vlctx_wf, h3⟩
+@[simp] theorem VContext.withMLC_self (c : VContext) : c.withMLC c.mlctx = c := by
+  simp [withMLC, c.lctx_eq]
+
+protected theorem RecM.WF.withLocalDecl {c : VContext} {m} [cwf : c.MLCWF m]
+    {s : VState} {f : Expr → RecM α} {Q name ty ty' bi}
+    (hty : (c.withMLC m).TrExpr ty ty')
+    (hty' : (c.withMLC m).IsType ty')
+    (H : ∀ id cwf' s', s.LE s' →
+      s'.ngen.Reserves id →
+      ¬s.ngen.Reserves id →
+      WF (c.withMLC (.vlam id name ty ty' bi m) (wf := cwf')) s' (f (.fvar id)) Q) :
+    (withLocalDecl name ty bi f).WF (c.withMLC m) s Q := by
+  simp [withLocalDecl, withFreshId]
+  refine .stateWF fun wf => ?_
+  refine fun _ mwf => mkFreshId.WF.bind fun id s le ⟨h0, h1⟩ wf' a s' e => ?_
+  have h1' := wf.find?_eq_none h1
+  have cwf' : c.MLCWF (.vlam ⟨id⟩ name ty ty' bi m) := ⟨cwf.1, h1', hty, hty'⟩
+  have : VState.WF (c.withMLC (.vlam ⟨id⟩ name ty ty' bi m)) s := {
+    ngen_wf := by simp [VContext.withMLC]; exact ⟨h0, wf'.ngen_wf⟩
+    trctx := wf.trctx.mkLocalDecl h1' hty hty'
   }
-  obtain ⟨s', hs1, hs2, wf', hs4⟩ := H _ h this a s' e
+  let ⟨s', hs1, hs2, wf', hs4⟩ := H _ _ _ le h0 h1 _ mwf this a s' e
   refine ⟨s', hs1, hs2, { wf with ngen_wf := ?_ }, hs4⟩
-  have := wf'.ngen_wf; simp [VContext.pushLDecl] at this; exact this.2
+  have := wf'.ngen_wf; simp [VContext.withMLC] at this; exact this.2
+
+@[simp] def MLCtx.mkForall (c : MLCtx) (n) (hn : n ≤ c.length) (e : Expr) : Expr :=
+  match n, c, hn, e with
+  | 0, _, _, e => e
+  | n+1, .vlam x name ty _ bi c, h, e =>
+    c.mkForall n (Nat.le_of_succ_le_succ h) (.forallE name ty (.abstractFVar x e) bi)
+termination_by structural n
+
+@[simp] def MLCtx.mkForall' (c : MLCtx) (n) (hn : n ≤ c.length) (e : VExpr) : VExpr :=
+  match n, c, hn, e with
+  | 0, _, _, e => e
+  | n+1, .vlam _ _ _ ty _ c, h, e =>
+    c.mkForall' n (Nat.le_of_succ_le_succ h) (.forallE ty e)
+termination_by structural n
+
+variable! (henv : VEnv.WF env) in
+theorem MLCtx.WF.mkForall_tr {c : MLCtx} (wf : c.WF env Us)
+    (tr : TrExpr env Us c.vlctx e e' ∧ env.IsType Us.length c.vlctx.toCtx e')
+    (n hn) :
+    TrExpr env Us (c.dropN n hn).vlctx (c.mkForall n hn e) (c.mkForall' n hn e') ∧
+    env.IsType Us.length (c.dropN n hn).vlctx.toCtx (c.mkForall' n hn e') := by
+  induction n generalizing c e e' with
+  | zero => exact tr
+  | succ n ih =>
+    let .vlam x name ty ty' bi c := c
+    refine ih wf.1 ⟨?_, .forallE wf.2.2.2 tr.2⟩ _
+    exact .forallE henv wf.1.tr.wf wf.2.2.2 tr.2 wf.2.2.1 (.abstract .zero tr.1)
+
+theorem MLCtx.fvarRevList_prefix (c : MLCtx)
+    {n hn} : c.fvarRevList n hn <+: c.vlctx.fvars := by
+  induction n generalizing c with
+  | zero => simp
+  | succ n ih =>
+    let .vlam x name ty ty' bi c := c
+    simp [ih]
+
+theorem MLCtx.WF.fvars_nodup : ∀ {c : MLCtx}, c.WF env Us → c.vlctx.fvars.Nodup
+  | .nil, _ => .nil
+  | .vlam _ _ _ _ _ c, ⟨h1, h2, h3, h4⟩ => by
+    simp [h1.fvars_nodup, h1.tr.find?_eq_none.1 h2]
+
+theorem MLCtx.WF.fvarRevList_nodup {c : MLCtx} (wf : c.WF env Us)
+    (n hn) : (c.fvarRevList n hn).Nodup :=
+  c.fvarRevList_prefix.sublist.nodup wf.fvars_nodup
+
+theorem MLCtx.WF.find?_eq_findDecl? {c : MLCtx} (wf : c.WF env Us) :
+    c.lctx.find? x = c.findDecl? x := sorry
+
+theorem MLCtx.WF.mkForall_eq {c : MLCtx} (wf : c.WF env Us) (n hn)
+    (harr : arr.toList.reverse = (c.fvarRevList n hn).map .fvar) :
+    c.lctx.mkForall' arr e = c.mkForall n hn e := by
+  have := congrArg (Array.mk ·.reverse) harr; simp at this
+  rw [LocalContext.mkForall', this, ← List.map_reverse, LocalContext.mkBinding'_eq,
+    LocalContext.mkBindingList_eq_fold, List.foldr_reverse]
+  · clear harr this
+    induction n generalizing c e with
+    | zero => simp [tr]
+    | succ n ih =>
+      let .vlam x name ty ty' bi c := c; simp
+      refine (List.foldl_congr fun _ _ h => ?_).trans <|
+        .trans (congrFun (congrArg _ ?_) _) (ih wf.1 _)
+      · refine LocalContext.mkBindingList1_congr ?_
+        rw [wf.find?_eq_findDecl?, wf.1.find?_eq_findDecl?, findDecl?, if_neg]
+        simp; rintro ⟨⟩
+        have := wf.fvarRevList_nodup (n+1) hn; simp_all
+      · simp [LocalContext.mkBindingList1, wf.find?_eq_findDecl?, findDecl?]
+  · intro _ h
+    exact wf.tr.find?_eq_some.2 ((MLCtx.fvarRevList_prefix ..).subset (List.mem_reverse.1 h))
+  · exact List.nodup_reverse.2 (wf.fvarRevList_nodup ..)
 
 namespace Inner
 
@@ -142,33 +307,74 @@ theorem ensureSortCore.WF {c : VContext} {s : VState} (he : c.TrExpr e e') :
       ∃ u, c.IsDefEqU e' (.sort u) ∧ c.TrExpr e1 (.sort u) :=
   sorry
 
+theorem checkLambda.loop.WF {c : VContext} {e₀ : Expr}
+    {m} [mwf : c.MLCWF m] {n} (hn : n ≤ m.length)
+    (hdrop : m.dropN n hn = c.mlctx)
+    (harr : arr.toList.reverse = (m.fvarRevList n hn).map .fvar)
+    (hr : e.FVarsIn s.ngen.Reserves ∧ ∀ v ∈ m.vlctx.fvars, s.ngen.Reserves v)
+    (ih : ∀ e' ty',
+      (c.withMLC m).TrExpr (e.instantiateList ((m.fvarRevList n hn).map .fvar)) e' →
+      (c.withMLC m).HasType e' ty' →
+      ∃ e₀', c.TrExpr e₀ e₀' ∧ c.HasType e₀' (m.mkForall' n hn ty')) :
+    (inferLambda.loop false arr e).WF (c.withMLC m) s (fun ty _ => ∃ e' ty',
+      c.TrExpr e₀ e' ∧ c.TrExpr ty ty' ∧ c.HasType e' ty') := by
+  unfold inferLambda.loop; split <;> simp only [pure_bind]
+  · rename_i name dom body bi
+    refine checkType.WF.bind fun uv _ le₁ ⟨dom', uv', h1, h2, h3⟩ => ?_
+    refine (ensureSortCore.WF h2).bind fun _ _ le₂ ⟨u, h4, h5⟩ => ?_
+    refine .stateWF fun wf => ?_
+    have domty := h3.defeqU_r c.venv_wf mwf.1.tr.wf.toCtx h4
+    have domty' : (c.withMLC m).IsType dom' := ⟨_, domty⟩
+    refine .withLocalDecl h1 domty' fun a mwf' s' le₃ res h6 => ?_
+    have h6' := wf.find?_eq_none h6
+    refine .stateWF fun wf' => ?_
+    refine checkLambda.loop.WF (mwf := mwf') (arr := arr.push _) (Nat.succ_le_succ hn)
+      (by simp [hdrop]) (by simp [harr]) ?_ ?_
+    · have := le₁.trans le₂ |>.trans le₃
+      simp [or_imp, forall_and, FVarsIn]
+      exact ⟨(this.reserves hr.1).2, res, fun _ h => this.reservesV (hr.2 _ h)⟩
+    intro e ty' h7 h9
+    dsimp [VContext.TrExpr, VContext.HasType] at h7 h9
+    simp [Expr.instantiateRev', Expr.instantiate', harr] at h1
+    simp [Expr.instantiateList_lam] at ih
+    conv at h7 => arg 4; exact (Expr.instantiateList_instantiate1_comm (by trivial)).symm
+    have h7 := h7.uninstantiate ((hr.1.2.instantiateList ?r).mono ?a)
+    case r => simp [FVarsIn]; exact fun _ h => hr.2 _ (m.fvarRevList_prefix.subset h)
+    case a => rintro _ h rfl; exact h6 <| (le₁.trans le₂).reservesV h
+    refine ih _ _ (.lam c.venv_wf mwf.1.tr.wf domty' h1 h7) (.lam domty h9)
+  · refine checkType.WF.bind fun ty _ _ ⟨e', ty', h1, h2, h3⟩ => ?_
+    refine .stateWF fun wf => .getLCtx <| .pure ?_
+    simp [Expr.instantiateRev', Expr.instantiate', harr] at h1
+    have ⟨e₀', h1', h2'⟩ := ih _ _ h1 h3
+    refine ⟨_, m.mkForall' n hn ty', h1', ?_, h2'⟩
+    simp [VContext.withMLC]; rw [mwf.1.mkForall_eq _ _ harr]
+    change TrExpr _ _ c.mlctx.vlctx ..; rw [← hdrop]
+    refine (mwf.1.mkForall_tr c.venv_wf ⟨?_, h3.isType c.venv_wf mwf.1.tr.wf.toCtx⟩ _ _).1
+    have : ty.Safe := sorry -- FIXME: I don't think this is provable
+    exact h2.cheapBetaReduce c.venv_wf wf.trctx.wf this m.noBV
+
+theorem checkLambda.WF
+    (h1 : e.FVarsIn s.ngen.Reserves) :
+    (inferLambda e false).WF c s (fun ty _ => ∃ e' ty',
+      c.TrExpr e e' ∧ c.TrExpr ty ty' ∧ c.HasType e' ty') :=
+  .stateWF fun wf =>
+  c.withMLC_self ▸ checkLambda.loop.WF (Nat.zero_le _) rfl rfl ⟨h1, wf.ngen_wf⟩
+    fun _ _ h1 h2 => ⟨_, h1, h2⟩
+
 theorem inferLambda.loop.WF
     (he : c.TrExpr e e')
     (hty : c.HasType e' ty') :
     (inferLambda.loop true fvars e).WF c s Q := by
   unfold inferLambda.loop; split
   · rename_i name dom body bi; simp
-    refine mkFreshId.WF.lift.bind fun a s' le ⟨res, h6⟩ => .getLCtx ?_
     refine .stateWF fun wf => ?_
     let ⟨_, .lam h1 h2 h3, _⟩ := he
     have := h2.trExpr c.venv_wf wf.trctx.wf
+    -- refine .withLocalDecl h1 ⟨_, h3.defeqU_r c.venv_wf wf.vlctx_wf h4⟩ fun a s' le res h6 => ?_
     -- refine RecM.WF.withLam res h6 h1 ⟨_, h3.defeqU_r c.venv_wf wf.vlctx_wf h4⟩ ?_
     -- exact inferLambda.loop.WF
     sorry
   · sorry
-
-theorem checkLambda.loop.WF {c₀ : VContext} {e₀ : Expr}
-    : (inferLambda.loop false fvars e).WF c s (fun ty _ => ∃ e' ty',
-      c₀.TrExpr e₀ e' ∧ c₀.TrExpr ty ty' ∧ c₀.HasType e' ty') := by
-  unfold inferLambda.loop; split <;> simp only [pure_bind] <;>
-    refine checkType.WF.bind fun ty _ _ ⟨ty', uv', h1, h2, h3⟩ => ?_
-  · refine (ensureSortCore.WF h2).bind fun _ _ _ ⟨u, h4, h5⟩ => ?_
-    refine mkFreshId.WF.lift.bind fun a s' le ⟨res, h6⟩ => .getLCtx ?_
-    refine .stateWF fun wf => ?_
-    refine RecM.WF.withLam res h6 h1 ⟨_, h3.defeqU_r c.venv_wf wf.vlctx_wf h4⟩ ?_
-    exact checkLambda.loop.WF
-  · refine .getLCtx <| .pure ?_
-    sorry
 
 theorem inferLambda.WF : (inferLambda e true).WF c s Q := by
   simp [inferLambda]
