Lean4Lean/Quot.lean
@@ -1,6 +1,7 @@
 import Batteries.Tactic.OpenPrivate
 import Lean4Lean.Environment.Basic
 import Lean4Lean.Expr
+import Lean4Lean.Instantiate
 import Lean4Lean.LocalContext
 
 namespace Lean4Lean
@@ -23,14 +24,14 @@ def checkEqType (env : Environment) : Except KernelException Unit := do
   let [eqRefl] := info.ctors | fail "unexpected number of constructors for 'Eq' type"
   ExprBuildT.run do
     withLocalDecl `α (.sort (.param u)) .implicit fun α => do
-      if info.type != ((← read).mkForall #[α] <| .arrow α <| .arrow α .prop) then
+      if info.type != ((← read).mkForall' #[α] <| .arrow α <| .arrow α .prop) then
         fail "'Eq' has an expected type"
     let info ← env.get eqRefl
     let [u] := info.levelParams
       | fail "unexpected number of universe params at 'Eq' type constructor"
     withLocalDecl `α (.sort (.param u)) .implicit fun α => do
       withLocalDecl `a α .default fun a => do
-        if info.type != ((← read).mkForall #[α, a] <| mkApp3 (.const ``Eq [.param u]) α a a) then
+        if info.type != ((← read).mkForall' #[α, a] <| mkApp3 (.const ``Eq [.param u]) α a a) then
           fail "unexpected type for 'Eq' type constructor"
 
 def Environment.addQuot (env : Environment) : Except KernelException Environment := do
@@ -43,13 +44,13 @@ def Environment.addQuot (env : Environment) : Except KernelException Environment
     -- constant Quot.{u} {α : Sort u} (r : α → α → Prop) : Sort u
     let env := add env <| .quotInfo {
       name := ``Quot, kind := .type, levelParams := [`u]
-      type := (← read).mkForall #[α, r] <| .sort u
+      type := (← read).mkForall' #[α, r] <| .sort u
     }
     withLocalDecl `a α .default fun a => do
       -- constant Quot.mk.{u} {α : Sort u} (r : α → α → Prop) (a : α) : @Quot.{u} α r
       return add env <| .quotInfo {
         name := ``Quot.mk, kind := .ctor, levelParams := [`u]
-        type := (← read).mkForall #[α, r, a] <| mkApp2 (.const ``Quot [u]) α r
+        type := (← read).mkForall' #[α, r, a] <| mkApp2 (.const ``Quot [u]) α r
       }
   withLocalDecl `r (.arrow α (.arrow α .prop)) .implicit fun r => do
   let quot_r := mkApp2 (.const ``Quot [u]) α r
@@ -60,23 +61,23 @@ def Environment.addQuot (env : Environment) : Except KernelException Environment
     withLocalDecl `b α .default fun b => do
     let rab := mkApp2 r a b
     let fa_eq_fb := mkApp3 (.const ``Eq [v]) β (.app f a) (.app f b)
-    let sanity := (← read).mkForall #[a, b] <| .arrow rab fa_eq_fb
+    let sanity := (← read).mkForall' #[a, b] <| .arrow rab fa_eq_fb
     -- constant Quot.lift.{u, v} {α : Sort u} {r : α → α → Prop} {β : Sort v} (f : α → β) :
     --   (∀ a b : α, r a b → f a = f b) → @Quot.{u} α r → β
     return add env <| .quotInfo {
       name := ``Quot.lift, kind := .lift, levelParams := [`u, `v]
-      type := (← read).mkForall #[α, r, β, f] <| .arrow sanity <| .arrow quot_r β
+      type := (← read).mkForall' #[α, r, β, f] <| .arrow sanity <| .arrow quot_r β
     }
   let quotMk_a := mkApp3 (.const ``Quot.mk [u]) α r a
   withLocalDecl `β (.arrow quot_r .prop) .implicit fun β => do
-  let all_quot := (← read).mkForall #[a] <| .app β quotMk_a
+  let all_quot := (← read).mkForall' #[a] <| .app β quotMk_a
   withLocalDecl `q quot_r .implicit fun q => do
   -- constant Quot.ind.{u} {α : Sort u} {r : α → α → Prop} {β : @Quot.{u} α r → Prop} :
   --   (∀ a : α, β (@Quot.mk.{u} α r a)) → ∀ q : @Quot.{u} α r, β q */
   let env := add env <| .quotInfo {
     name := ``Quot.ind, kind := .ind, levelParams := [`u]
-    type := (← read).mkForall #[α, r, β] <|
-      .forallE `mk all_quot ((← read).mkForall #[q] <| .app β q) .default
+    type := (← read).mkForall' #[α, r, β] <|
+      .forallE `mk all_quot ((← read).mkForall' #[q] <| .app β q) .default
   }
   return markQuotInit env
 
